feat(library/init/meta/interactive): `simp` and `unfold` can unfold projection applications
@Armael: we finally can write `simp [proj]` to unfold the `proj`
projection application.

Remark: we still need to add similar support for `dsimp`.

src/library/tactic/simplify.cpp
@@ -38,6 +38,7 @@ Author: Daniel Selsam, Leonardo de Moura
 #include "library/vm/vm_list.h"
 #include "library/vm/vm_nat.h"
 #include "library/vm/vm_name.h"
+#include "library/tactic/eqn_lemmas.h"
 #include "library/tactic/tactic_state.h"
 #include "library/tactic/ac_tactics.h"
 #include "library/tactic/app_builder_tactics.h"
@@ -1070,7 +1071,31 @@ optional<pair<simp_result, bool>> simplify_fn::pre(expr const &, optional<expr> 
     return no_ext_result();
 }
 
+static optional<simp_result> to_opt_simp_result(optional<expr> const & e) {
+    if (!e) return optional<simp_result>();
+    return optional<simp_result>(*e);
+}
+
+optional<simp_result> simplify_fn::unfold_step(expr const & e) {
+    if (m_to_unfold.empty())
+        return optional<simp_result>();
+    if (!is_app(e) && !is_constant(e))
+        return optional<simp_result>();
+    expr const & fn = get_app_fn(e);
+    if (!is_constant(fn) || !m_to_unfold.contains(const_name(fn)))
+        return optional<simp_result>();
+    type_context::transparency_scope scope(m_ctx, transparency_mode::Instances);
+    optional<expr> new_e;
+    if (is_projection(m_ctx.env(), const_name(fn))) {
+        return to_opt_simp_result(m_ctx.reduce_projection(e));
+    } else {
+        return to_opt_simp_result(unfold_term(m_ctx.env(), e));
+    }
+}
+
 optional<pair<simp_result, bool>> simplify_fn::post(expr const & e, optional<expr> const &) {
+    if (auto r = unfold_step(e))
+        return to_ext_result(*r);
     simp_result r = rewrite(e);
     if (r.get_new() != e) {
         return to_ext_result(r);
