library/init/meta/converter/interactive.lean
@@ -41,7 +41,7 @@ conv.whnf
 
 meta def dsimp (no_dflt : parse only_flag) (es : parse opt_qexpr_list) (attr_names : parse with_ident_list)
                (ids : parse without_ident_list) (cfg : tactic.dsimp_config := {}) : conv unit :=
-do s ← tactic.mk_simp_set no_dflt attr_names es ids,
+do (s, u) ← tactic.mk_simp_set no_dflt attr_names es ids,
    conv.dsimp (some s) cfg
 
 meta def trace_lhs : conv unit :=
@@ -111,9 +111,9 @@ do (r, lhs, _) ← tactic.target_lhs_rhs,
 meta def simp (no_dflt : parse only_flag) (hs : parse opt_qexpr_list) (attr_names : parse with_ident_list)
               (ids : parse without_ident_list) (cfg : tactic.simp_config_ext := {})
               : conv unit :=
-do s ← tactic.mk_simp_set no_dflt attr_names hs ids,
+do (s, u) ← tactic.mk_simp_set no_dflt attr_names hs ids,
    (r, lhs, rhs) ← tactic.target_lhs_rhs,
-   (new_lhs, pr) ← tactic.simplify s [] lhs cfg.to_simp_config r cfg.discharger,
+   (new_lhs, pr) ← tactic.simplify s u lhs cfg.to_simp_config r cfg.discharger,
    update_lhs new_lhs pr,
    return ()
 
