tests/lean/run/and_rec_code_gen_issue.lean
@@ -74,7 +74,7 @@ lemma init_mem_inv : ∀ n (b : buffer nat), n < b.size → (init_mem n).pre b
 | (nat.succ n) b h :=
   have n < b.size, from nat.lt_of_succ_lt h,
   begin
-    dunfold init_mem has_bind.and_then bind has_bind.bind hoare_state.bind, simp,
+    unfold init_mem has_bind.and_then bind has_bind.bind hoare_state.bind, simp,
     split,
     {unfold hoare_state.assign, simp, exact h},
     {intros _ _,
